      %%%%%%%%%%%%%%%%%%%%%%%%%%%%%%%%%%%%%%%%%%%%%%%%%%%%%%%%%%%%%%%%%%%%%%%%%%%%%%%%%%%%%%%
      %                         vidu                                                        %
      %%%%%%%%%%%%%%%%%%%%%%%%%%%%%%%%%%%%%%%%%%%%%%%%%%%%%%%%%%%%%%%%%%%%%%%%%%%%%%%%%%%%%%%
      
          \begin{vd}
            Giải phương trình: $ \sqrt{2x-3} = x-3 $

          \end{vd}
          \begin{center}

            Giải:
         \end{center}
          Phương trình đã cho tương đương với: \\
         $
            \begin{cases}
                x - 3 \geq 0 \\
                2x- 3 = (x-3)^2
            \end{cases}
          $ 
        $    \Leftrightarrow $
          $
            \begin{cases}
                x \geq 3 \\
                2x - 3 = x^2 -6x +9
            \end{cases}
          $ \\
        $    \Leftrightarrow $
         $
            \begin{cases}
                x  \geq 3 \\
                x^2 - 8x + 12 =0
            \end{cases}
          $ 
        $    \Leftrightarrow $
         $
            \begin{cases}
                x  \geq 3 \\
                \left[ \begin{array} {l}
                    x=6 \\ 
                    x=2
                  \end{array}
                \right.
                
            \end{cases}
          $ 
        $    \Leftrightarrow $
        $
            x=6.
        $
         \\        
         Kết luận: vậy phương trình có một nghiệm là $x=6$
