
         
      %%%%%%%%%%%%%%%%%%%%%%%%%%%%%%%%%%%%%%%%%%%%%%%%%%%%%%%%%%%%%%%%%%%%%%%%%%%%%%%%%%%%%%%
      %                         vidu                                                        %
      %%%%%%%%%%%%%%%%%%%%%%%%%%%%%%%%%%%%%%%%%%%%%%%%%%%%%%%%%%%%%%%%%%%%%%%%%%%%%%%%%%%%%%%
      
          \begin{vd}
              Giải phương trình: $\sqrt{3x+4} - \sqrt{2x+1} = \sqrt{x+3}$
          \end{vd}
          \begin{center}

            Giải:
         \end{center}
         Điều kiện: $ \begin{cases}
                            3x + 4 \geq 0 \\
                            2x + 1 \geq 0 \\
                            \sqrt{3x+4} \geq \sqrt{2x+1}\\
                            x+3 \geq 0
                      \end{cases}
                    $
                    $\Leftrightarrow
                    \begin{cases}
                        x \geq - \dfrac{4}{3} \\
                        x \geq -\dfrac{1}{2} \\
                        3x +4 \geq 2x +1 \\
                        x \geq 3
                    \end{cases}
                    $
                    $\Leftrightarrow
                    \begin{cases}
                        x \geq -\frac{4}{3} \\
                        x \geq -\frac{1}{2} \\
                        x \geq -3 \\
                        x \geq -3
                    \end{cases}
                    $
                    $\Leftrightarrow x \geq -\frac{1}{2}$ \\
                    Với điều kiện trên phương trình tương đương \\
                    $
                    \sqrt{3x+4} = \sqrt{x+3} + \sqrt{2x+1}
                    $ \\
                    $\Leftrightarrow
                    3x+4 = 3x +4 + 2\sqrt{(x+3)(2x+1)}
                    $ \\
                    $\Leftrightarrow 
                    \left[
                        \begin{array}{l}
                            x=-3 \\
                            x=-\frac{1}{2}
                        \end{array}
                    \right.
                    $ \\
                    So sánh với điều kiện ta được nghiệm phương trình là $x=-\frac{1}{2}$.

