%%%%%%%%%%%%%%%%%%%%%%%%%%%%%%%%%%%%%%%%%%%%%%%%%%%%%%%%%%%%%%%%%%%%%%%%%%%%%%%%
%			                 vi du				       %
%%%%%%%%%%%%%%%%%%%%%%%%%%%%%%%%%%%%%%%%%%%%%%%%%%%%%%%%%%%%%%%%%%%%%%%%%%%%%%%%
\begin{vd}
  Giải phương trình: $ 2\left(\sqrt{2(2+x)}+2\sqrt{2-x}\right) = \sqrt{9x^2+16} $
\end{vd}
\begin{center}
    Giải:
\end{center}

Điều kiện: $ -2 \leq x \leq 2 $ \\
Với điều kiện trên phương trình tương đương : \\
$ 8(2+x) + 16\sqrt{2(4-x^2)} + 16(2-x) = 9x^2+16 $ \\
$ \Leftrightarrow 
    9x^2 +8x - 32 = 16 \sqrt{2(4-x^2}
$ //
$ \Leftrightarrow 
    (9x^2 +8x -32)^2 = 512(4 -x^2)
$\\
$\Leftrightarrow 
    81x^4 +144x^2 -512x -1024=0
$\\
$\Leftrightarrow 
    (9x^2-32)(9x^2 +16x+32)=0
    $\\
$\Leftrightarrow 
x=\pm \dfrac{\sqrt{32}}{3}
$\\
Thử lại ta được nghiệm của phương trình : $x=\dfrac{\sqrt{32}}{3}$
